positive_div: split out other example

theories/Dot/examples/positive_div.v
@@ -1,3 +1,4 @@
+(** * Semantic typing for positive numbers and division. *)
 From iris.proofmode Require Import tactics.
 From D.pure_program_logic Require Import lifting adequacy.
 From iris.program_logic Require Import ectxi_language.
@@ -18,33 +19,27 @@ Implicit Types (v w : vl) (d : dm) (ds : dms).
 
 Import hoas.syn.
 
-Module Import examplesBodies.
-Import hoasNotation.
+(** ** Example code. *)
+Section examplesBodies.
+  Import hoasNotation.
 
-Definition posModT := μ: self, {@
-  type "Pos" >: ⊥ <: 𝐙;
-  val "mkPos" : 𝐙 →: self @; "Pos";
-  val "div" : 𝐙 →: self @; "Pos" →: 𝐙
-}.
+  Definition hdivV := λ: m n, m `div` (htskip n).
+  Definition hmkPosBodyV (n : hvl) := htif (n > 0) n hloopTm.
+  Definition hmkPosV := λ: n, hmkPosBodyV n.
 
-Definition hdivV := λ: m n, m `div` (htskip n).
-Definition hmkPosBodyV (n : hvl) := htif (n > 0) n hloopTm.
-Definition hmkPosV := λ: n, hmkPosBodyV n.
+  Definition hposModV s : hvl := ν: _ , {@
+    type "Pos" = ([]; s);
+    val "mkPos" = hmkPosV;
+    val "div" = hdivV
+  }.
 
-Definition hposModV s : hvl := ν: _ , {@
-  type "Pos" = ([]; s);
-  val "mkPos" = hmkPosV;
-  val "div" = hdivV
-}.
-
-Definition hminiV s := ν: _, {@
-  type "A" = ([]; s);
-  val "n" = 2
-}.
-
+  (** Actual type *)
+  Definition posModT := μ: self, {@
+    type "Pos" >: ⊥ <: 𝐙;
+    val "mkPos" : 𝐙 →: self @; "Pos";
+    val "div" : 𝐙 →: self @; "Pos" →: 𝐙
+  }.
 End examplesBodies.
-
-Module examples.
 
 Local Hint Constructors bin_op_syntype cond_bin_op_syntype : core.
 Local Hint Extern 1000 => lia : core.
@@ -54,10 +49,10 @@ Ltac wp_bin := iApply wp_wand; [wp_bin_base | iIntros].
 Import stamp_transfer.
 
 Local Open Scope Z_scope.
+
 (* Generic useful lemmas — not needed for fundamental theorem,
     but very useful for examples. *)
 Section helpers.
-
   Context `{HdlangG: !dlangG Σ}.
 
   Lemma alloc {s sγ} φ : sγ !! s = None → allGs sγ ==∗ s ↝n[ 0 ] φ.
@@ -116,37 +111,22 @@ Ltac valMember ρ :=
   iApply V_TVMem_I; [solve_fv_congruence|naive_solver|
     rewrite -ietp_value; iIntros (ρ)].
 
-Section s_is_pos.
-
-Context `{HdlangG: !dlangG Σ}.
-Context (s: stamp).
-
 Definition pos v := ∃ n, v = vint n ∧ n > 0.
-Definition ipos: oltyO Σ 0 := olty0 (λI ρ v, ⌜ pos v ⌝).
+Definition ipos {Σ}: oltyO Σ 0 := olty0 (λI ρ v, ⌜ pos v ⌝).
 
-Definition Hs : iProp Σ := s ↝n[ 0 ] ipos.
-Lemma allocHs sγ:
-  sγ !! s = None → allGs sγ ==∗ Hs.
-Proof. exact (alloc ipos). Qed.
+Definition s_is_pos `{!dlangG Σ} s : iProp Σ := s ↝n[ 0 ] ipos.
 
 Section div_example.
-  (* Arguments dlang_ectx_lang : simpl never.
-  Arguments dlang_ectxi_lang : simpl never. *)
+  Context `{HdlangG: !dlangG Σ} `{SwapPropI Σ}.
+  Context (s: stamp).
 
-  Lemma pos_wp ρ v : ipos vnil ρ v ⊢ WP v > 0 {{ w, w ≡ vbool true }}.
-  Proof. iDestruct 1 as %(n & -> & ?). by iApply wp_ge. Qed.
+  Definition posModV : vl := hposModV s.
 
-  Context `{SwapPropI Σ}.
-  Lemma loopSemT: ⊢ WP hloopTm {{ _, False }}.
-  Proof using Type*.
-    iDestruct (fundamental_typed (loopTyp []) with "[]") as "H".
-    iApply wellMappedφ_empty.
-    iSpecialize ("H" $! ids with "[//]").
-    by rewrite hsubst_id /=.
-  Qed.
+  Notation Hs := (s_is_pos s).
+  Lemma allocHs sγ:
+    sγ !! s = None → allGs sγ ==∗ Hs.
+  Proof. exact (alloc ipos). Qed.
 
-  Section useHoas.
-  Import hoasNotation.
   Lemma wp_if_ge (n : Z) :
     ⊢ WP hmkPosBodyV n {{ w, ⌜ w = n ∧ n > 0 ⌝}}.
   Proof using Type*.
@@ -157,20 +137,7 @@ Section div_example.
     iApply wp_wand; [iApply loopSemT | naive_solver].
   Qed.
 
-  Lemma wp_if_ge' (n : Z) :
-    ⊢ WP tif (n > 0) (1 `div` n) hloopTm {{ w, ⟦ 𝐙 ⟧ ids w ∧ ⌜ n > 0 ⌝}}.
-  Proof using Type*.
-    wp_bind (IfCtx _ _).
-    wp_bin; ev; simplify_eq/=.
-    case_decide; rewrite -wp_pure_step_later //; iNext.
-    - wp_bin. naive_solver.
-    - iApply wp_wand; [iApply loopSemT | naive_solver].
-  Qed.
-  End useHoas.
-
   (** We assume [Hs] throughout the rest of the section. *)
-
-  Definition posModV : vl := hposModV s.
 
   Lemma sToIpos : Hs -∗ dtysem [] s ↗n[ 0 ] hoEnvD_inst [] ipos.
   Proof. by iApply dm_to_type_intro. Qed.
@@ -262,137 +229,8 @@ Section div_example.
   Qed.
 End div_example.
 
-Section small_ex.
-  (* Generic useful lemmas — not needed for fundamental theorem,
-     but very useful for examples. *)
-
-  (** Under Iris assumption [Hs], [miniV.A] points to [ipos]. *)
-  Import DBNotation.
-
-  Definition miniVT1Body : ty := {@
-    type "A" >: ⊥ <: 𝐙;
-    val "n" : p0 @; "A"
-  }.
-  Definition miniVT1 := μ miniVT1Body.
-  Definition miniV : vl := hminiV s.
-
-
-  (** Yes, miniV has a valid type member. *)
-  Lemma vHasA0typ: Hs -∗ [] ⊨ miniV : type "A" >: ⊥ <: 𝐙.
-  Proof.
-    iIntros "#Hs".
-    iApply (T_Sub (i := 0) (T1 := μ {@ type "A" >: ⊥ <: 𝐙})).
-    iApply T_Obj_I.
-    iApply D_Cons; [done| by iApply sHasA'|].
-    iSplit; [iIntros "!%"|iIntros "!> ** //"].
-    repeat constructor; exact: not_elem_of_nil.
-    iApply Sub_Trans.
-    iApply (Mu_Sub {@ type "A" >: ⊥ <: 𝐙}).
-    iApply sAnd1_Sub.
-  Qed.
-  (* This works. Crucially, we use T_Mu_I to introduce the object type.
-     This way, we can inline the object in the type selection.
-     This cannot be done using T_Obj_I directly.
-     However, this is closer to how typechecking in Scala
-     actually works.
-     XXX: also, maybe this *could* be done with T_Obj_I with
-     a precise type? That'd be a more correct derivation.
-   *)
-  Lemma vHasA1t : Hs -∗ [] ⊨ miniV : miniVT1.
-  Proof.
-    rewrite -(T_Mu_I _ miniV).
-    iIntros "#Hs /=".
-    iApply sT_And_I; first by [iApply vHasA0typ].
-    iApply sT_And_I; first last.
-    - iApply (T_Sub (i := 0) (T2 := TTop)); last by iApply sSub_Top.
-      by iApply vHasA0typ.
-    - rewrite -setp_value_eq /= /iPPred_car /=.
-      have Hev2: pos (vint 2) by rewrite /pos; eauto.
-      iIntros (_).
-
-      repeat (repeat iExists _; repeat iSplit; rewrite ?path_wp_pv_eq //);
-        try by [|iApply dm_to_type_intro].
-  Qed.
-
-  (*
-    A different approach would be to type the object using T_Obj_I
-    with an object type [U] with member [TTMem "A" ipos ipos].
-    We could then upcast the object. But type U is not syntactic,
-    so we can't express this yet using the existing typing
-    lemmas.
-    And if we use T_Obj_I on the final type, then [this.A]
-    is overly abstract when we try proving that [this.n : this.A];
-    see concretely below.
-  *)
-  Definition miniVT2Body : ty := {@
-    type "A" >: ⊥ <: 𝐙;
-    val "n" : TLater (p0 @; "A")
-  }.
-  Definition miniVT2 := μ miniVT2Body.
-
-  Definition sminiVT2Body : oltyO Σ 0 :=
-    oAnd (cTMem "A" oBot (oPrim tint))
-      (oAnd (cVMem "n" (oLater (oSel p0 "A")))
-      oTop).
-  Goal V⟦miniVT2Body⟧ = sminiVT2Body. done. Abort.
-  Definition sminiVT2 := oMu sminiVT2Body.
-
-  Definition sminiVT2ConcrBody : cltyO Σ :=
-    cAnd (cTMem "A" ipos ipos)
-      (cAnd (cVMem "n" (oLater (oSel p0 "A")))
-      cTop).
-  Definition sminiVT2Concr := oMu sminiVT2ConcrBody.
-
-  Lemma sT_Var0 {Γ T}
-    (Hx : Γ !! 0%nat = Some T):
-    (*──────────────────────*)
-    ⊢ Γ s⊨ x0 : T.
-  Proof. rewrite -(hsubst_id T). apply (sT_Var Hx). Qed.
-
-  (* This works! But we get a weaker type, because we're using typing rules
-  for recursive objects on a not-really-recursive one. *)
-  Lemma vHasA2t `{SwapPropI Σ}: Hs -∗ [] s⊨ miniV : sminiVT2.
-  Proof.
-    iIntros "#Hs".
-    iApply (sT_Sub (i := 0) (T1 := sminiVT2Concr)); first last.
-    - iApply sMu_Sub_Mu; rewrite /sminiVT2ConcrBody /miniVT1Body oLaterN_0.
-      iApply sSub_And; last iApply sSub_And; last iApply sSub_Top.
-    + iApply sSub_Trans; first iApply sAnd1_Sub.
-      iApply sTyp_Sub_Typ; [iApply sBot_Sub | iApply Sub_later_ipos_nat].
-    + iApply sSub_Trans; first iApply sAnd2_Sub.
-      iApply sAnd1_Sub.
-    - rewrite /miniV /sminiVT2Concr /sminiVT2ConcrBody.
-      iApply sT_Obj_I.
-      iApply sD_Cons; first done.
-      iApply (sD_Typ_Abs ipos); [iApply sSub_Refl..|by iExists _; iFrame "Hs"].
-      iApply sD_Cons; [done| |iApply sD_Nil].
-      iApply sD_Val.
-      iApply (sT_Sub (i := 0) (T1 := ipos)).
-      rewrite setp_value /ipos /pos; iIntros "!> %ρ _ /= !%". naive_solver.
-      iApply sSub_Trans; first iApply sSub_Add_Later.
-      iApply sSub_Trans; first iApply sSub_Add_Later.
-      iApply sSub_Later_Sub.
-      iApply sSub_Sel.
-      iApply sP_Later.
-      iApply sP_Val.
-      iApply (sT_Sub (i := 0)).
-      by iApply sT_Var0.
-      iApply sSub_Later_Sub.
-      iApply sAnd1_Sub.
-  Qed.
-End small_ex.
-End s_is_pos.
-
-Lemma miniVSafe (s : stamp): safe (miniV s).
-Proof.
-  eapply (safety_dot_sem dlangΣ (T := miniVT1))=>*.
-  by rewrite (allocHs s) // -vHasA1t.
-Qed.
-
 Lemma posModVSafe (s : stamp): safe (posModV s).
 Proof.
   eapply (safety_dot_sem dlangΣ (T := posModT))=>*.
   by rewrite (allocHs s) // -posModTy.
 Qed.
-
-End examples.
