tests/test_used_axioms.v
@@ -1,13 +1,14 @@
 From D Require Import prelude.
 From D.Dot Require Import fundamental.
-From D.Dot.examples Require positive_div from_pdot_mutual_rec_sem.
+From D.Dot.examples Require positive_div small_sem_ex from_pdot_mutual_rec_sem.
 
 Print Assumptions type_soundness.
 Print Assumptions path_normalization.
-Print Assumptions positive_div.examples.miniVSafe.
-Print Assumptions positive_div.examples.posModVSafe.
+Print Assumptions small_sem_ex.miniVSafe.
+Print Assumptions positive_div.posModVSafe.
 Print Assumptions from_pdot_mutual_rec_sem.pcoreSafe.
 
-From D.Dot.examples Require list.
+From D.Dot.examples Require list from_pdot_mutual_rec.
 
 Print Assumptions list.clListTypNat3.
+Print Assumptions from_pdot_mutual_rec.fromPDotPaperTyp.
