theories/Dot/examples/small_sem_ex.v
@@ -1,0 +1,155 @@
+(** * Exercise: Semantic typing for positive numbers (smallest example). *)
+From iris.proofmode Require Import tactics.
+From D.pure_program_logic Require Import lifting adequacy.
+From iris.program_logic Require Import ectxi_language.
+
+From D Require Import swap_later_impl.
+From D.Dot Require Import scala_lib hoas ex_utils storeless_typing_ex_utils ex_iris_utils.
+
+From D.Dot Require Import unary_lr
+  binding_lr tsel_lr no_binding_lr defs_lr prims_lr.
+From D.Dot Require Import tdefs_lr.
+From D.Dot Require Import skeleton fundamental syn_lemmas.
+
+From D.Dot.examples Require Import positive_div.
+Import dlang_adequacy.
+
+Set Suggest Proof Using.
+Set Default Proof Using "Type".
+
+Implicit Types (v w : vl) (d : dm) (ds : dms).
+
+Import hoas.syn.
+
+(** ** Example code. *)
+Section examplesBodies.
+  Import hoasNotation.
+  Definition hminiV s := ν: _, {@
+    type "A" = ([]; s);
+    val "n" = 2
+  }.
+
+  Definition hminiVT1 := μ: x, {@
+    type "A" >: ⊥ <: 𝐙;
+    val "n" : x @; "A"
+  }.
+End examplesBodies.
+
+Section small_ex.
+  Context `{HdlangG: !dlangG Σ} `{SwapPropI Σ}.
+  Context (s: stamp).
+
+  Notation Hs := (s_is_pos s).
+  Definition miniV : vl := hminiV s.
+  (** Under Iris assumption [Hs], [miniV.A] points to [ipos]. *)
+
+  (** Show that miniV has a valid type member. *)
+  Lemma vHasA0typ: Hs -∗ [] ⊨ miniV : type "A" >: ⊥ <: 𝐙.
+  Proof.
+    iIntros "#Hs".
+    iApply (T_Sub (i := 0) (T1 := μ {@ type "A" >: ⊥ <: 𝐙})).
+    iApply T_Obj_I.
+    iApply D_Cons; [done| by iApply sHasA'|].
+    iSplit; [iIntros "!%"|iIntros "!> ** //"]; first naive_solver.
+    iApply Sub_Trans.
+    iApply (Mu_Sub {@ type "A" >: ⊥ <: 𝐙}).
+    iApply sAnd1_Sub.
+  Qed.
+  (* This works. Crucially, we use T_Mu_I to introduce the object type.
+     This way, we can inline the object in the type selection.
+     This cannot be done using T_Obj_I directly.
+     However, this is closer to how typechecking in Scala
+     actually works.
+     XXX: also, maybe this *could* be done with T_Obj_I with
+     a precise type? That'd be a more correct derivation.
+   *)
+  Lemma vHasA1t : Hs -∗ [] ⊨ miniV : hminiVT1.
+  Proof.
+    rewrite -(T_Mu_I _ miniV).
+    iIntros "#Hs /=".
+    iApply sT_And_I; first by [iApply vHasA0typ].
+    iApply sT_And_I; first last.
+    - iApply (T_Sub (i := 0) (T2 := TTop)); last by iApply sSub_Top.
+      by iApply vHasA0typ.
+    - rewrite -setp_value_eq /= /iPPred_car /=.
+      have Hev2: pos (vint 2) by rewrite /pos; eauto with lia.
+      iIntros (_).
+
+      repeat (repeat iExists _; repeat iSplit; rewrite ?path_wp_pv_eq //);
+        try by [|iApply dm_to_type_intro].
+  Qed.
+
+  (*
+    A different approach would be to type the object using T_Obj_I
+    with an object type [U] with member [TTMem "A" ipos ipos].
+    We could then upcast the object. But type U is not syntactic,
+    so we can't express this yet using the existing typing
+    lemmas.
+    And if we use T_Obj_I on the final type, then [this.A]
+    is overly abstract when we try proving that [this.n : this.A];
+    see concretely below.
+  *)
+  Definition miniVT2Body : ty := {@
+    type "A" >: ⊥ <: 𝐙;
+    val "n" : TLater (p0 @; "A")
+  }.
+  Definition miniVT2 := μ miniVT2Body.
+
+  Definition sminiVT2Body : oltyO Σ 0 :=
+    oAnd (cTMem "A" oBot (oPrim tint))
+      (oAnd (cVMem "n" (oLater (oSel p0 "A")))
+      oTop).
+  Goal V⟦miniVT2Body⟧ = sminiVT2Body. done. Abort.
+
+  Definition sminiVT2ConcrBody : cltyO Σ :=
+    cAnd (cTMem "A" ipos ipos)
+      (cAnd (cVMem "n" (oLater (oSel p0 "A")))
+      cTop).
+  Definition sminiVT2Concr := oMu sminiVT2ConcrBody.
+
+  Lemma sT_Var0 {Γ T}
+    (Hx : Γ !! 0%nat = Some T):
+    (*──────────────────────*)
+    ⊢ Γ s⊨ x0 : T.
+  Proof. rewrite -(hsubst_id T). apply (sT_Var Hx). Qed.
+
+  (* The next lemma [ demonstrates an alternative typing derivation,
+  using gDOT rules
+   But we get a weaker type, because we're using typing rules
+  for recursive objects on a not-really-recursive one. *)
+  Lemma vHasA2t `{SwapPropI Σ}: Hs -∗ [] ⊨ miniV : miniVT2.
+  Proof.
+    iIntros "#Hs".
+    iApply (sT_Sub (i := 0) (T1 := sminiVT2Concr)); first last.
+    - iApply sMu_Sub_Mu; rewrite /sminiVT2ConcrBody oLaterN_0.
+      iApply sSub_And; last iApply sSub_And; last iApply sSub_Top.
+    + iApply sSub_Trans; first iApply sAnd1_Sub.
+      iApply sTyp_Sub_Typ; [iApply sBot_Sub | iApply Sub_later_ipos_nat].
+    + iApply sSub_Trans; first iApply sAnd2_Sub.
+      iApply sAnd1_Sub.
+    - rewrite /miniV /hminiV /sminiVT2Concr /sminiVT2ConcrBody.
+      iApply sT_Obj_I.
+      iApply sD_Cons; first done.
+      iApply (sD_Typ_Abs ipos); [iApply sSub_Refl..|by iExists _; iFrame "Hs"].
+      iApply sD_Cons; [done| |iApply sD_Nil].
+      iApply sD_Val.
+      iApply (sT_Sub (i := 0) (T1 := ipos)).
+      rewrite setp_value /ipos /pos; iIntros "!> %ρ _ /= !%". naive_solver.
+      iApply sSub_Trans; first iApply sSub_Add_Later.
+      iApply sSub_Trans; first iApply sSub_Add_Later.
+      iApply sSub_Later_Sub.
+      iApply sSub_Sel.
+      iApply sP_Later.
+      iApply sP_Val.
+      iApply (sT_Sub (i := 0)).
+      by iApply sT_Var0.
+      iApply sSub_Later_Sub.
+      iApply sAnd1_Sub.
+  Qed.
+End small_ex.
+
+Lemma miniVSafe (s : stamp): safe (miniV s).
+Proof.
+  eapply (safety_dot_sem dlangΣ (T := hminiVT1))=>*.
+  by rewrite (allocHs s) // -vHasA1t.
+Qed.
